Define Galois adjoints between FL and RTMax

RT-FL/RT.thy
@@ -10,7 +10,15 @@ datatype 'e rtrefusal = RefNil ("\<bullet>\<^sub>\<R>\<^sub>\<T>") | RefSet "'e 
 
 datatype 'e rttrace  = RTRefusal "'e rtrefusal" ("\<langle>_\<rangle>\<^sub>\<R>\<^sub>\<T>") | RTEvent "'e rtrefusal" "'e" "'e rttrace" ("_ #\<^sub>\<R>\<^sub>\<T> _ #\<^sub>\<R>\<^sub>\<T> _")
 
+fun in_rtrefusal :: "'e \<Rightarrow> 'e rtrefusal \<Rightarrow> bool" (infix "\<in>\<^sub>\<R>\<^sub>\<T>" 50)  where
+  "e \<in>\<^sub>\<R>\<^sub>\<T> \<bullet>\<^sub>\<R>\<^sub>\<T> = False" |
+  "e \<in>\<^sub>\<R>\<^sub>\<T> [X]\<^sub>\<R>\<^sub>\<T> = (e \<in> X)"
+
 type_synonym 'e rtprocess = "'e rttrace set"
+
+fun rtWF :: "'e rttrace \<Rightarrow> bool" where
+  "rtWF \<langle>X\<rangle>\<^sub>\<R>\<^sub>\<T> = True" |
+  "rtWF (X #\<^sub>\<R>\<^sub>\<T> e #\<^sub>\<R>\<^sub>\<T> \<rho>) = (\<not> e \<in>\<^sub>\<R>\<^sub>\<T> X \<and> rtWF \<rho>)"
 
 section \<open>Healthiness Conditions\<close>
 
@@ -33,6 +41,29 @@ fun leq_rttrace :: "'e rttrace \<Rightarrow> 'e rttrace \<Rightarrow> bool" (inf
   "( [X]\<^sub>\<R>\<^sub>\<T> #\<^sub>\<R>\<^sub>\<T> a #\<^sub>\<R>\<^sub>\<T> \<rho>) \<le>\<^sub>\<R>\<^sub>\<T> ( \<bullet>\<^sub>\<R>\<^sub>\<T> #\<^sub>\<R>\<^sub>\<T> b #\<^sub>\<R>\<^sub>\<T> \<sigma>)   = False" |
   "( x #\<^sub>\<R>\<^sub>\<T> a #\<^sub>\<R>\<^sub>\<T> \<rho>)     \<le>\<^sub>\<R>\<^sub>\<T> \<langle>y\<rangle>\<^sub>\<R>\<^sub>\<T>                = False"
 
+lemma leq_rttrace_refl: "x \<le>\<^sub>\<R>\<^sub>\<T> x"
+  by (induct x, case_tac x, auto, case_tac x1a, auto)
+
+lemma leq_rttrace_trans: "\<And>y. x \<le>\<^sub>\<R>\<^sub>\<T> y \<Longrightarrow> y \<le>\<^sub>\<R>\<^sub>\<T> z \<Longrightarrow> x \<le>\<^sub>\<R>\<^sub>\<T> z"
+  apply (induct x z rule:leq_rttrace.induct, auto)
+  apply (case_tac y, auto, case_tac x1, auto)
+  apply (case_tac y, auto, case_tac x1, auto)
+  apply (case_tac y, auto, case_tac x1, auto, case_tac x21, auto)
+  apply (case_tac y, auto, case_tac x1, auto, case_tac x21, auto)
+  apply (case_tac y, auto, case_tac x21, auto)
+  apply (case_tac y, auto, case_tac x21, auto)
+  apply (case_tac y, auto, case_tac x21, auto)
+  apply (case_tac y, auto, case_tac x21, auto)
+  apply (case_tac y, auto, case_tac x21, auto)
+  apply (case_tac y, auto, case_tac x21, auto)
+  apply (case_tac y, auto, case_tac x21, auto)
+  apply (case_tac y, auto, case_tac x21, auto)
+  apply (case_tac y, auto, (case_tac ya, auto)+)
+  done
+
+lemma leq_rttrace_antisym: "x \<le>\<^sub>\<R>\<^sub>\<T> y \<Longrightarrow> y \<le>\<^sub>\<R>\<^sub>\<T> x \<Longrightarrow> x = y"
+  by (induct x y rule:leq_rttrace.induct, auto, case_tac \<sigma>, auto, case_tac x1, auto)
+
 definition RT1 :: "'e rtprocess \<Rightarrow> bool" where
   "RT1 P = (\<forall> \<rho> \<sigma>. \<sigma> \<in> P \<and> \<rho> \<le>\<^sub>\<R>\<^sub>\<T> \<sigma> \<longrightarrow> \<rho> \<in> P)"
 
@@ -41,10 +72,41 @@ subsection \<open>RT2\<close>
 datatype 'e rttrace_tail = RTEmptyTail | RTEventTail 'e "'e rttrace" (infixr "##\<^sub>\<R>\<^sub>\<T>" 65)
 datatype 'e rttrace_init = RTEmptyInit | RTEventInit "'e rtrefusal" 'e "'e rttrace_init"
 
+fun rttrace_init_eq :: "'e rttrace_init \<Rightarrow> 'e rttrace_init \<Rightarrow> bool" where
+  "rttrace_init_eq RTEmptyInit RTEmptyInit = False" |
+  "rttrace_init_eq RTEmptyInit (RTEventInit x e \<rho>) = False" |
+  "rttrace_init_eq (RTEventInit x e \<rho>) RTEmptyInit = False" |
+  "rttrace_init_eq (RTEventInit x e \<rho>) (RTEventInit y f \<sigma>) = rttrace_init_eq \<rho> \<sigma>"
+
+fun rttrace2init :: "'e rttrace \<Rightarrow> 'e rttrace_init" where
+  "rttrace2init \<langle>y\<rangle>\<^sub>\<R>\<^sub>\<T> = RTEmptyInit" |
+  "rttrace2init (x #\<^sub>\<R>\<^sub>\<T> a #\<^sub>\<R>\<^sub>\<T> \<rho>) = RTEventInit x a (rttrace2init \<rho>)"
+
 fun rttrace_with_refusal :: "'e rttrace_init \<Rightarrow> 'e rtrefusal \<Rightarrow> 'e rttrace_tail \<Rightarrow> 'e rttrace" ("_ @\<^sub>\<R>\<^sub>\<T> \<langle>_\<rangle>\<^sub>\<R>\<^sub>\<T> @\<^sub>\<R>\<^sub>\<T> _" [65, 65, 65] 65) where
   "((RTEventInit x a \<rho>) @\<^sub>\<R>\<^sub>\<T> \<langle>y\<rangle>\<^sub>\<R>\<^sub>\<T> @\<^sub>\<R>\<^sub>\<T> \<sigma>) = (x #\<^sub>\<R>\<^sub>\<T> a #\<^sub>\<R>\<^sub>\<T> (\<rho> @\<^sub>\<R>\<^sub>\<T> \<langle>y\<rangle>\<^sub>\<R>\<^sub>\<T> @\<^sub>\<R>\<^sub>\<T> \<sigma>))" |
   "(RTEmptyInit @\<^sub>\<R>\<^sub>\<T> \<langle>y\<rangle>\<^sub>\<R>\<^sub>\<T> @\<^sub>\<R>\<^sub>\<T> (RTEventTail b \<sigma>)) = (y #\<^sub>\<R>\<^sub>\<T> b #\<^sub>\<R>\<^sub>\<T> \<sigma>)" |
   "(RTEmptyInit @\<^sub>\<R>\<^sub>\<T> \<langle>b\<rangle>\<^sub>\<R>\<^sub>\<T> @\<^sub>\<R>\<^sub>\<T> RTEmptyTail) = \<langle>b\<rangle>\<^sub>\<R>\<^sub>\<T>"
+
+fun leq_rttrace_init :: "'e rttrace_init \<Rightarrow> 'e rttrace_init \<Rightarrow> bool" where
+  "leq_rttrace_init RTEmptyInit \<rho> = True" |
+  "leq_rttrace_init (RTEventInit X e \<rho>) RTEmptyInit = False" |
+  "leq_rttrace_init (RTEventInit \<bullet>\<^sub>\<R>\<^sub>\<T> e \<rho>) (RTEventInit Y f \<sigma>) = (e = f \<and> leq_rttrace_init \<rho> \<sigma>)" |
+  "leq_rttrace_init (RTEventInit [X]\<^sub>\<R>\<^sub>\<T> e \<rho>) (RTEventInit \<bullet>\<^sub>\<R>\<^sub>\<T> f \<sigma>) = False" |
+  "leq_rttrace_init (RTEventInit [X]\<^sub>\<R>\<^sub>\<T> e \<rho>) (RTEventInit [Y]\<^sub>\<R>\<^sub>\<T> f \<sigma>) = (X \<subseteq> Y \<and> e = f \<and> leq_rttrace_init \<rho> \<sigma>)"
+
+lemma rttrace_with_refusal_eq1:
+  "\<rho> @\<^sub>\<R>\<^sub>\<T> \<langle>X\<rangle>\<^sub>\<R>\<^sub>\<T> @\<^sub>\<R>\<^sub>\<T> RTEmptyTail = \<sigma> @\<^sub>\<R>\<^sub>\<T> \<langle>Y\<rangle>\<^sub>\<R>\<^sub>\<T> @\<^sub>\<R>\<^sub>\<T> RTEmptyTail \<Longrightarrow> \<rho> = \<sigma>"
+  by (induct \<rho> \<sigma> rule: rttrace_init_eq.induct, auto)
+
+lemma rttrace_with_refusal_eq2:
+  "\<rho> @\<^sub>\<R>\<^sub>\<T> \<langle>X\<rangle>\<^sub>\<R>\<^sub>\<T> @\<^sub>\<R>\<^sub>\<T> RTEmptyTail = \<sigma> @\<^sub>\<R>\<^sub>\<T> \<langle>Y\<rangle>\<^sub>\<R>\<^sub>\<T> @\<^sub>\<R>\<^sub>\<T> RTEmptyTail \<Longrightarrow> X = Y"
+  by (induct \<rho> \<sigma> rule: rttrace_init_eq.induct, auto)
+
+lemma rttrace_with_refusal_eq3:
+  "\<rho> @\<^sub>\<R>\<^sub>\<T> \<langle>X\<rangle>\<^sub>\<R>\<^sub>\<T> @\<^sub>\<R>\<^sub>\<T> e ##\<^sub>\<R>\<^sub>\<T> \<langle>x\<rangle>\<^sub>\<R>\<^sub>\<T> = \<sigma> @\<^sub>\<R>\<^sub>\<T> \<langle>Y\<rangle>\<^sub>\<R>\<^sub>\<T> @\<^sub>\<R>\<^sub>\<T> f ##\<^sub>\<R>\<^sub>\<T> \<langle>y\<rangle>\<^sub>\<R>\<^sub>\<T> \<Longrightarrow> \<rho> = \<sigma>"
+  apply (induct \<rho> \<sigma> rule: rttrace_init_eq.induct, auto)
+  apply (metis (full_types) rttrace.simps(4) rttrace_with_refusal.elims rttrace_with_refusal.simps(2))
+  using rttrace_with_refusal.elims by blast
 
 definition RT2 :: "'e rtprocess \<Rightarrow> bool" where
   "RT2 P = (\<forall> \<rho> \<sigma> X Y. 
@@ -68,6 +130,14 @@ definition RT4 :: "'e rtevent rtprocess \<Rightarrow> bool" where
     \<rho> @\<^sub>\<R>\<^sub>\<T> \<langle>x\<rangle>\<^sub>\<R>\<^sub>\<T> @\<^sub>\<R>\<^sub>\<T> TickRT ##\<^sub>\<R>\<^sub>\<T> \<langle>y\<rangle>\<^sub>\<R>\<^sub>\<T> \<in> P
       \<longrightarrow> x = \<bullet>\<^sub>\<R>\<^sub>\<T> \<and> \<rho> @\<^sub>\<R>\<^sub>\<T> \<langle>\<bullet>\<^sub>\<R>\<^sub>\<T>\<rangle>\<^sub>\<R>\<^sub>\<T> @\<^sub>\<R>\<^sub>\<T> TickRT ##\<^sub>\<R>\<^sub>\<T> \<langle>[UNIV]\<^sub>\<R>\<^sub>\<T>\<rangle>\<^sub>\<R>\<^sub>\<T> \<in> P)"
 
+subsection \<open>RT\<close>
+
+definition RT :: "'e rtevent rtprocess \<Rightarrow> bool" where
+  "RT P = ((\<forall>x\<in>P. rtWF x) \<and> MRT0 P \<and> RT1 P \<and> RT2 P \<and> RT3 P \<and> RT4 P)"
+
+definition refinesRT :: "'e rtprocess \<Rightarrow> 'e rtprocess \<Rightarrow> bool" (infix "\<sqsubseteq>\<^sub>\<R>\<^sub>\<T>" 50) where
+  "P \<sqsubseteq>\<^sub>\<R>\<^sub>\<T> Q = (Q \<subseteq> P)"
+
 section \<open>Maximal Healthiness Conditions\<close>
 
 subsection \<open>RTM1 (replaces RT1)\<close>
@@ -78,11 +148,50 @@ fun leq_rttrace_max :: "'e rttrace \<Rightarrow> 'e rttrace \<Rightarrow> bool" 
   "\<langle> [X]\<^sub>\<R>\<^sub>\<T>\<rangle>\<^sub>\<R>\<^sub>\<T>           \<le>\<^sub>\<R>\<^sub>\<T>\<^sub>\<M> \<langle> \<bullet>\<^sub>\<R>\<^sub>\<T>\<rangle>\<^sub>\<R>\<^sub>\<T>             = False" |
   "\<langle> [X]\<^sub>\<R>\<^sub>\<T>\<rangle>\<^sub>\<R>\<^sub>\<T>           \<le>\<^sub>\<R>\<^sub>\<T>\<^sub>\<M> ( [Y]\<^sub>\<R>\<^sub>\<T> #\<^sub>\<R>\<^sub>\<T> b #\<^sub>\<R>\<^sub>\<T> \<sigma>) = (X = Y)" |
   "\<langle> [X]\<^sub>\<R>\<^sub>\<T>\<rangle>\<^sub>\<R>\<^sub>\<T>           \<le>\<^sub>\<R>\<^sub>\<T>\<^sub>\<M> ( \<bullet>\<^sub>\<R>\<^sub>\<T> #\<^sub>\<R>\<^sub>\<T> b #\<^sub>\<R>\<^sub>\<T> \<sigma>)   = False" |
-  "( \<bullet>\<^sub>\<R>\<^sub>\<T> #\<^sub>\<R>\<^sub>\<T> a #\<^sub>\<R>\<^sub>\<T> \<rho>)   \<le>\<^sub>\<R>\<^sub>\<T>\<^sub>\<M> ( \<bullet>\<^sub>\<R>\<^sub>\<T> #\<^sub>\<R>\<^sub>\<T> b #\<^sub>\<R>\<^sub>\<T> \<sigma>)   = (a = b \<and> \<rho> \<le>\<^sub>\<R>\<^sub>\<T> \<sigma>)" |
-  "( \<bullet>\<^sub>\<R>\<^sub>\<T> #\<^sub>\<R>\<^sub>\<T> a #\<^sub>\<R>\<^sub>\<T> \<rho>)   \<le>\<^sub>\<R>\<^sub>\<T>\<^sub>\<M> ( [Y]\<^sub>\<R>\<^sub>\<T> #\<^sub>\<R>\<^sub>\<T> b #\<^sub>\<R>\<^sub>\<T> \<sigma>) = (a = b \<and> \<rho> \<le>\<^sub>\<R>\<^sub>\<T> \<sigma>)" |
-  "( [X]\<^sub>\<R>\<^sub>\<T> #\<^sub>\<R>\<^sub>\<T> a #\<^sub>\<R>\<^sub>\<T> \<rho>) \<le>\<^sub>\<R>\<^sub>\<T>\<^sub>\<M> ( [Y]\<^sub>\<R>\<^sub>\<T> #\<^sub>\<R>\<^sub>\<T> b #\<^sub>\<R>\<^sub>\<T> \<sigma>) = (X = Y \<and> a = b \<and> \<rho> \<le>\<^sub>\<R>\<^sub>\<T> \<sigma>)" |
+  "( \<bullet>\<^sub>\<R>\<^sub>\<T> #\<^sub>\<R>\<^sub>\<T> a #\<^sub>\<R>\<^sub>\<T> \<rho>)   \<le>\<^sub>\<R>\<^sub>\<T>\<^sub>\<M> ( \<bullet>\<^sub>\<R>\<^sub>\<T> #\<^sub>\<R>\<^sub>\<T> b #\<^sub>\<R>\<^sub>\<T> \<sigma>)   = (a = b \<and> \<rho> \<le>\<^sub>\<R>\<^sub>\<T>\<^sub>\<M> \<sigma>)" |
+  "( \<bullet>\<^sub>\<R>\<^sub>\<T> #\<^sub>\<R>\<^sub>\<T> a #\<^sub>\<R>\<^sub>\<T> \<rho>)   \<le>\<^sub>\<R>\<^sub>\<T>\<^sub>\<M> ( [Y]\<^sub>\<R>\<^sub>\<T> #\<^sub>\<R>\<^sub>\<T> b #\<^sub>\<R>\<^sub>\<T> \<sigma>) = (a = b \<and> \<rho> \<le>\<^sub>\<R>\<^sub>\<T>\<^sub>\<M> \<sigma>)" |
+  "( [X]\<^sub>\<R>\<^sub>\<T> #\<^sub>\<R>\<^sub>\<T> a #\<^sub>\<R>\<^sub>\<T> \<rho>) \<le>\<^sub>\<R>\<^sub>\<T>\<^sub>\<M> ( [Y]\<^sub>\<R>\<^sub>\<T> #\<^sub>\<R>\<^sub>\<T> b #\<^sub>\<R>\<^sub>\<T> \<sigma>) = (X = Y \<and> a = b \<and> \<rho> \<le>\<^sub>\<R>\<^sub>\<T>\<^sub>\<M> \<sigma>)" |
   "( [X]\<^sub>\<R>\<^sub>\<T> #\<^sub>\<R>\<^sub>\<T> a #\<^sub>\<R>\<^sub>\<T> \<rho>) \<le>\<^sub>\<R>\<^sub>\<T>\<^sub>\<M> ( \<bullet>\<^sub>\<R>\<^sub>\<T> #\<^sub>\<R>\<^sub>\<T> b #\<^sub>\<R>\<^sub>\<T> \<sigma>)   = False" |
   "( x #\<^sub>\<R>\<^sub>\<T> a #\<^sub>\<R>\<^sub>\<T> \<rho>)     \<le>\<^sub>\<R>\<^sub>\<T>\<^sub>\<M> \<langle>y\<rangle>\<^sub>\<R>\<^sub>\<T>                = False"
+
+lemma leq_rttrace_max_refl: "x \<le>\<^sub>\<R>\<^sub>\<T>\<^sub>\<M> x"
+  by (induct x, case_tac x, auto, case_tac x1a, auto)
+
+lemma leq_rttrace_max_trans: "\<And>y. x \<le>\<^sub>\<R>\<^sub>\<T>\<^sub>\<M> y \<Longrightarrow> y \<le>\<^sub>\<R>\<^sub>\<T>\<^sub>\<M> z \<Longrightarrow> x \<le>\<^sub>\<R>\<^sub>\<T>\<^sub>\<M> z"
+  apply (induct x z rule:leq_rttrace.induct, auto)
+  apply (case_tac y, auto, case_tac x1, auto)
+  apply (case_tac y, auto, case_tac x1, auto)
+  apply (case_tac y, auto, case_tac x1, auto)
+  apply (case_tac y, auto, case_tac x1, auto, case_tac x21, auto)
+  apply (case_tac y, auto, case_tac x1, auto, case_tac x21, auto)
+  apply (case_tac y, auto, case_tac x1, auto, case_tac x21, auto)
+  apply (case_tac y, auto, case_tac x21, auto)
+  apply (case_tac y, auto, case_tac x21, auto)
+  apply (case_tac y, auto, case_tac x21, auto)
+  apply (case_tac y, auto, case_tac x21, auto)
+  apply (case_tac y, auto, case_tac x21, auto)
+  apply (case_tac y, auto, case_tac x21, auto)
+  apply (case_tac y, auto, case_tac x21, auto)
+  apply (case_tac y, auto, case_tac x21, auto)
+  apply (case_tac y, auto, case_tac x21, auto)
+  apply (case_tac y, auto, (case_tac ya, auto)+)
+  done
+
+lemma leq_rttrace_max_antisym: "x \<le>\<^sub>\<R>\<^sub>\<T>\<^sub>\<M> y \<Longrightarrow> y \<le>\<^sub>\<R>\<^sub>\<T>\<^sub>\<M> x \<Longrightarrow> x = y"
+  by (induct x y rule:leq_rttrace.induct, auto, case_tac \<sigma>, auto, case_tac x1, auto)
+
+fun leq_rttrace_init_max :: "'e rttrace_init \<Rightarrow> 'e rttrace_init \<Rightarrow> bool" where
+  "leq_rttrace_init_max RTEmptyInit \<rho> = True" |
+  "leq_rttrace_init_max (RTEventInit X e \<rho>) RTEmptyInit = False" |
+  "leq_rttrace_init_max (RTEventInit \<bullet>\<^sub>\<R>\<^sub>\<T> e \<rho>) (RTEventInit Y f \<sigma>) = (e = f \<and> leq_rttrace_init_max \<rho> \<sigma>)" |
+  "leq_rttrace_init_max (RTEventInit [X]\<^sub>\<R>\<^sub>\<T> e \<rho>) (RTEventInit \<bullet>\<^sub>\<R>\<^sub>\<T> f \<sigma>) = False" |
+  "leq_rttrace_init_max (RTEventInit [X]\<^sub>\<R>\<^sub>\<T> e \<rho>) (RTEventInit [Y]\<^sub>\<R>\<^sub>\<T> f \<sigma>) = (X \<subseteq> Y \<and> e = f \<and> leq_rttrace_init_max \<rho> \<sigma>)"
+
+fun leq_rttrace_rttrace_init_max :: "'e rttrace \<Rightarrow> 'e rttrace_init \<Rightarrow> bool" where
+  "leq_rttrace_rttrace_init_max \<langle>x\<rangle>\<^sub>\<R>\<^sub>\<T> RTEmptyInit = False" |
+  "leq_rttrace_rttrace_init_max (v #\<^sub>\<R>\<^sub>\<T> va #\<^sub>\<R>\<^sub>\<T> vb) RTEmptyInit = False" |
+  "leq_rttrace_rttrace_init_max \<langle>vc\<rangle>\<^sub>\<R>\<^sub>\<T> (RTEventInit v va vb) = (vc = v)" |
+  "leq_rttrace_rttrace_init_max (v #\<^sub>\<R>\<^sub>\<T> va #\<^sub>\<R>\<^sub>\<T> vb) (RTEventInit vc vd ve) = (v = vc \<and> va = vd \<and> leq_rttrace_rttrace_init_max vb ve)"
 
 definition RTM1 :: "'e rtprocess \<Rightarrow> bool" where
   "RTM1 P = (\<forall> \<rho> \<sigma>. \<sigma> \<in> P \<and> \<rho> \<le>\<^sub>\<R>\<^sub>\<T>\<^sub>\<M> \<sigma> \<longrightarrow> \<rho> \<in> P)"
@@ -91,3 +200,10 @@ subsection \<open>RTM2 (replaces RT2)\<close>
 
 definition RTM2 :: "'e rtprocess \<Rightarrow> bool" where
   "RTM2 P = (\<forall> \<rho> X e. \<rho> @\<^sub>\<R>\<^sub>\<T> \<langle>[X]\<^sub>\<R>\<^sub>\<T>\<rangle>\<^sub>\<R>\<^sub>\<T> @\<^sub>\<R>\<^sub>\<T> RTEmptyTail \<in> P \<and> e \<notin> X \<longrightarrow> \<rho> @\<^sub>\<R>\<^sub>\<T> \<langle>[X]\<^sub>\<R>\<^sub>\<T>\<rangle>\<^sub>\<R>\<^sub>\<T> @\<^sub>\<R>\<^sub>\<T> e ##\<^sub>\<R>\<^sub>\<T> \<langle>\<bullet>\<^sub>\<R>\<^sub>\<T>\<rangle>\<^sub>\<R>\<^sub>\<T> \<in> P)"
+
+subsection \<open>RTM\<close>
+
+definition RTM :: "'e rtevent rtprocess \<Rightarrow> bool" where
+  "RTM P = ((\<forall>x\<in>P. rtWF x) \<and> MRT0 P \<and> RTM1 P \<and> RTM2 P \<and> RT3 P \<and> RT4 P)"
+
+end
